\documentclass{article}
\usepackage{custom}
\usepackage{shortex}
\title{ 8-4 }

\begin{document}

\maketitle
\pagebreak


\subsubsection*{ 3 a) }

Let $T: P_2 \to P_2$ be the linear operator defined by

$$
T \left(a _ {0} + a _ {1} x + a _ {2} x ^ {2}\right) = a _ {0} + a _ {1} (x - 1) + a _ {2} (x - 1) ^ {2}
$$

Find the matrix for $T$ relative to the standard basis $B = \{1,x,x^2\}$ for $P_{2}$
\vfill


\subsubsection*{ b) }

Verify that the matrix $[T]_B$ obtained in part (a) satisfies Formula (8) for every vector $\mathbf{x} = a_0 + a_1x + a_2x^2$ in $P_{2}$
\vfill

\pagebreak

\subsubsection*{ 4 a) }

Let $T: R^2 \to R^2$ be the linear operator defined by

$$
T \left(\left[ \begin{array}{l} x _ {1} \\ x _ {2} \end{array} \right]\right) = \left[ \begin{array}{l} x _ {1} - x _ {2} \\ x _ {1} + x _ {2} \end{array} \right]
$$

and let $B = \{\mathbf{u}_1,\mathbf{u}_2\}$ be the basis for which

$$
\mathbf {u} _ {1} = \left[ \begin{array}{l} 1 \\ 1 \end{array} \right] \quad \text {a n d} \quad \mathbf {u} _ {2} = \left[ \begin{array}{l} - 1 \\ 0 \end{array} \right]
$$

Find $[T]_B$
\vfill


\subsubsection*{ b) }

Verify that Formula (8) holds for every vector $\mathbf{x}$ in $R^2$
\vfill

\pagebreak

\subsubsection*{ 5 a) }

Let $T: R^2 \to R^3$ be defined by

$$
T \left(\left[ \begin{array}{c} x _ {1} \\ x _ {2} \end{array} \right]\right) = \left[ \begin{array}{c} x _ {1} + 2 x _ {2} \\ - x _ {1} \\ 0 \end{array} \right]
$$

Find the matrix $[T]_{B',B}$ relative to the bases $B = \{\mathbf{u}_1,\mathbf{u}_2\}$ and $B^{\prime} = \{\mathbf{v}_1,\mathbf{v}_2,\mathbf{v}_3\}$ where

$$
\begin{array}{l} \mathbf {u} _ {1} = \left[ \begin{array}{l} 1 \\ 3 \end{array} \right], \quad \mathbf {u} _ {2} = \left[ \begin{array}{l} - 2 \\ 4 \end{array} \right] \\ \mathbf {v} _ {1} = \left[ \begin{array}{l} 1 \\ 1 \\ 1 \end{array} \right], \quad \mathbf {v} _ {2} = \left[ \begin{array}{l} 2 \\ 2 \\ 0 \end{array} \right], \quad \mathbf {v} _ {3} = \left[ \begin{array}{l} 3 \\ 0 \\ 0 \end{array} \right] \\ \end{array}
$$
\vfill


\subsubsection*{ b) }

Verify that Formula (5) holds for every vector in $R^2$
\vfill

\pagebreak

\subsubsection*{ 7 a) }

Let $T: P_2 \to P_2$ be the linear operator defined by

$$
\begin{array}{l} T (p (x)) = p (2 x + 1), \text {t h a t i s}, \\ T \left(c _ {0} + c _ {1} x + c _ {2} x ^ {2}\right) = c _ {0} + c _ {1} (2 x + 1) + c _ {2} (2 x + 1) ^ {2} \\ \end{array}
$$

Find $[T]_B$ with respect to the basis $B = \{1, x, x^2\}$ .
\vfill


\subsubsection*{ b) }

Use the three-step procedure illustrated in Example 2 to compute $T(2 - 3x + 4x^2)$ .
\vfill

\pagebreak

\subsubsection*{ c) }

Check the result obtained in part (b) by computing $T(2 - 3x + 4x^2)$ directly.
\vfill


\subsubsection*{ 9 a) }

Let $\mathbf{v}_1 = \begin{bmatrix} 1 \\ 3 \end{bmatrix}$ and $\mathbf{v}_2 = \begin{bmatrix} -1 \\ 4 \end{bmatrix}$ , and let $A = \begin{bmatrix} 1 & 3 \\ -2 & 5 \end{bmatrix}$ be the matrix for $T: R^2 \to R^2$ relative to the basis $B = \{\mathbf{v}_1, \mathbf{v}_2\}$ .

Find $[T(\mathbf{v}_1)]_B$ and $[T(\mathbf{v}_2)]_B$
\vfill

\pagebreak

\subsubsection*{ b) }

Find $T(\mathbf{v}_1)$ and $T(\mathbf{v}_2)$
\vfill


\subsubsection*{ c) }

Find a formula for $T\left(\left[ \begin{array}{l}x_{1}\\ x_{2} \end{array} \right]\right)$
\vfill

\pagebreak

\subsubsection*{ d) }

Use the formula obtained in (c) to compute $T\left(\left[ \begin{array}{l}1\\ 1 \end{array} \right]\right)$

\pagebreak
\vfill


\subsubsection*{ Answers }

3. (a) $ \begin{bmatrix} 1 & -1 & 1 \\ 0 & 1 & -2 \\ 0 & 0 & 1 \end{bmatrix} $

5. (a) $ \begin{bmatrix} 0 & 0 \\ -\frac{1}{2} & 1 \\ \frac{8}{3} & \frac{4}{3} \end{bmatrix} $

7. (a) $\left[ \begin{array}{lll}1 & 1 & 1\\ 0 & 2 & 4\\ 0 & 0 & 4 \end{array} \right]$

(b),(c) $3 + 10x + 16x^{2}$

9. (a) $[T(\mathbf{v}_1)]_B = \begin{bmatrix} 1 \\ -2 \end{bmatrix}; [T(\mathbf{v}_2)]_B = \begin{bmatrix} 3 \\ 5 \end{bmatrix}$

(b) $T(\mathbf{v}_1) = \left[ \begin{array}{l}3\\ -5 \end{array} \right];T(\mathbf{v}_2) = \left[ \begin{array}{l} - 2\\ 29 \end{array} \right]$

(c) $T\left(\left[ \begin{array}{l}x_{1}\\ x_{2} \end{array} \right]\right) = \left[ \begin{array}{cc}\frac{18}{7} & \frac{1}{7}\\ -\frac{107}{7} & \frac{24}{7} \end{array} \right]\left[ \begin{array}{l}x_{1}\\ x_{2} \end{array} \right]$

(d) $T\left(\left[ \begin{array}{l}1\\ 1 \end{array} \right]\right) = \left[ \begin{array}{l}\frac{19}{7}\\ -\frac{83}{7} \end{array} \right]$
\vfill

\pagebreak

\end{document}