# Chapter 6-3

1-21 odd

In Problems 1â€“14 for each differential equation find two linearly independent power series solutions about the ordinary point x=0.

1. $y'' = xy$ 
3. $y'' - 2xy' + y = 0$ 
5. $y'' + x^2y' + xy = 0$ 
7. $(x - 1)y'' + y' = 0$ 
9. $(x^2 - 1)y'' + 4xy' + 2y = 0$ 
11. $(x^2 + 2)y'' + 3xy' - y = 0$ 
13. $y'' - (x + 1)y' - y = 0$ 

In Problems 15-18 use the power series method to solve the given differential equation subject to the indicated initial conditions. 

15. $(x - 1)y'' - xy' + y = 0, \quad y(0) = -2, y'(0) = 6$ 
17. $y'' - 2xy' + 8y = 0, \quad y(0) = 3, y'(0) = 0$ 

In Problems 19-22 use the procedure illustrated in Example 9 to find two power series solutions of the given differential equation about the ordinary point $x = 0$. 

19. $y'' + (sin x)y = 0$ 
21. $y'' + e^{-x}y = 0$ 

\pagebreak

## Answers

1. $y_{1}(x) = c_{0}\left[1 + \frac{1}{3 \cdot 2} x^{3} + \frac{1}{6 \cdot 5 \cdot 3 \cdot 2} x^{6}\right.$ $+ \frac{1}{9 \cdot 8 \cdot 6 \cdot 5 \cdot 3 \cdot 2} x^{9} + \dots$ 
$$y_{2}(x) = c_{1}\left[x + \frac{1}{4 \cdot 3} x^{4} + \frac{1}{7 \cdot 6 \cdot 4 \cdot 3} x^{7} + \dots\right.$$


3. $$y_{1}(x) = c_{0}\left[1 - \frac{1}{27} x^{3} - \frac{3}{4!} x^{4} - \frac{21}{6!} x^{6} - \dots\right]$$
$$y_{2}(x) = c_{1}\left[x + \left(\frac{1}{3!} x^{3} + \frac{5}{5!} x^{5} + \frac{45}{7!} x^{7} + \dots\right)\right.$$


5. $y_{1}(x) = c_{0}\left[1 - \frac{1}{3!} x^{3} + \frac{4^{2}}{6!} x^{6} - \frac{7^{2} \cdot 4^{2}}{9!} x^{9} + \dots\right]$ 
$$y_{2}(x) = c_{1}\left[x - \frac{2^{2}}{4!} x^{4} + \frac{5^{2} \cdot 2^{2}}{7!} x^{7} - \frac{8^{2} \cdot 5^{2} \cdot 2^{2}}{10!} x^{10} + \dots\right]$$

7. $y_{1}(x) = c_{0}; \quad y_{2}(x) = c_{1} \sum_{n=1}^{\infty} \frac{1}{n} x^{n}$ 

9. $y_{1}(x) = c_{0} \sum_{n=0}^{\infty} x^{2n}; \quad y_{2}(x) = c_{1} \sum_{n=0}^{\infty} x^{2n+1}$ 

11. $y_{1}(x) = c_{0}\left[1 + \frac{x^{2}}{4} - \frac{7}{4 \cdot 4!} x^{4} + \frac{23 \cdot 7}{8 \cdot 6!} x^{6} - \dots\right]$ 
$$y_{2}(x) = c_{1}\left[x - \left(\frac{1}{6} x^{3} + \frac{14}{2 \cdot 5!} x^{5} - \frac{34 \cdot 14}{4 \cdot 7!} x^{7} - \dots\right)\right]$$

13. $y_{1}(x) = c_{0}\left[1 + \frac{\frac{1}{2!} x^{2}}{x^{2}} + \frac{\frac{1}{3!} x^{3}}{x^{3}} + \frac{\frac{1}{4!} x^{4}}{x^{4}} + \dots\right]$ 
$$y_{2}(x) = c_{1}\left[x + \tfrac{1}{2!} x^{2} + \tfrac{1}{3!} x^{3} + \tfrac{1}{4!} x^{4} + \dots\right]$$

15. $y(x) = -2\left[1 + \frac{1}{2!} x^{2} + \frac{1}{3!} x^{3} + \frac{1}{4!} x^{4} + \dots\right] + 6x$ 
$$= 8x - 2e^{x}$$

17. $y(x) = 3 - 12x^{2} + 4x^{4}$ 

19. $y_{1}(x) = c_{0}\left[1 - \frac{\frac{1}{6} x^{3}}{x^{3}} + \frac{1}{120} x^{5} + \dots\right]$ 
$$y_{2}(x) = c_{1}\left[x - \tfrac{1}{12} x^{4} + \tfrac{1}{180} x^{6} + \dots\right]$$

21. $y_{1}(x) = c_{0}\left[1 - \frac{x^{2}}{6} + \frac{x^{3}}{6} - \frac{x^{4}}{40} + \dots\right]$
