
\documentclass[fleqn]{article}
\usepackage{amsmath}
\usepackage{shortex}
\title{2.4}
\begin{document}

\maketitle
\pagebreak
 "Determine whether the given equation is exacit. If it is find the  solve."

\subparagraph{1}

\[
(2x - 1)dx + (3y + 7)dy = 0
\]
\vfill



\subparagraph{3}

\[
(5x + 4y)dx + (4x - 8y^3)dy = 0(5x + 4y)dx + (4x - 8y^3)dy = 0
\]
\vfill


\pagebreak


\subparagraph{5}

\[
(2y^2x - 3)dx + (2yx^2 + 4)dy = 0
\]
\vfill



\subparagraph{7}

\[
(x + y)(x - y)dx + x(x - 2y)dy = 0
\]
\vfill


\pagebreak


\subparagraph{9}

\[
(y^3 - y^2 \sin x - x)dx + (3xy^2 + 2y \cos x)dy = 0
\]
\vfill



\subparagraph{13}

\[
x\frac{dy}{dx} = 2xe^x - y + 6x^2
\]
\vfill


\pagebreak


\subparagraph{17}

\[
\left(x^2y^3 - \frac{1}{1 + 9x^2}\right)\frac{dx}{dy} + x^3y^2 = 0
\]
\vfill



\subparagraph{21}

\[
(1 - 2x^2 - 2y) \frac{dy}{dx} = 4x^3 + 4xy
\]
\vfill


\pagebreak
 Solve the differential equation with the inital condition.

\subparagraph{25}

\[
(x + y)^{2} dx + (2xy + x^{2} - 1)dy = 0, \quad y(1) = 1
\]
\vfill



\subparagraph{29}

\[
(y^{2} \cos x - 3x^{2}y - 2x)dx + (2y \sin x - x^{3} + \ln y)dy = 0, \quad y(0) = e
\]
\vfill


\pagebreak
 Find the value of $k$ so that the given differential equation is exact.

\subparagraph{33}

\[
(2xy^{2} + ye^{x})dx + (2x^{2}y + ke^{x} - 1)dy = 0
\]
\vfill

 "Solve the differential equation by verifying that the indicated fuction $\mu (x  y)$ is an inegrating factor."

\subparagraph{37}

\[
6xy dx + (4y + 9x^2) dy = 0, \mu(x, y) = y^2
\]
\vfill


\pagebreak


\subparagraph{41}

\[
(2y^2 + 3x) dx + 2xy dy = 0, \mu(x, y) = x
\]
\vfill


\pagebreak
\subsection*{Answers:}


\subparagraph{1}

\[
x^2 - x + \frac{3}{2}y^2 + 7y = c 
\]
\vfill



\subparagraph{3}

\[
\frac{5}{2}x^2 + 4xy - 2y^4 = c
\]
\vfill



\subparagraph{5}

\[
x^2y^2 - 3x + 4y = c 
\]
\vfill



\subparagraph{7}

\[
not exact, but is homogeneous
\]
\vfill



\subparagraph{9}

\[
xy^3 + y^2 \cos x - \frac{1}{2}x^2 = c 
\]
\vfill



\subparagraph{13}

\[
xy - 2xe^x + 2e^x - 2x^3 = c
\]
\vfill



\subparagraph{17}

\[
x^3y^3 - \tan^{-1}3x = c
\]
\vfill



\subparagraph{21}

\[
y - 2x^2y - y^2 - x^4 = c
\]
\vfill



\subparagraph{25}

\[
\frac{1}{3}x^3 + x^2y + xy^2 - y = \frac{4}{3}
\]
\vfill



\subparagraph{29}

\[
y^2 \sin x - x^3y - x^2 + y \ln y - y = 0
\]
\vfill



\subparagraph{33}

\[
k = 1
\]
\vfill



\subparagraph{37}

\[
M(x, y) = 6xy^3 \\ N(x, y) = 4y^3 + 9x^2y^2 \\ \frac{\partial M}{\partial y} = 18xy^2 = \frac{\partial N}{\partial x} \\ Solution is 3x^2y^3 + y^4 = c.
\]
\vfill



\subparagraph{41}

\[
M(x, y) = 2xy^2 + 3x^2 \\ N(x, y) = 2x^2y \\ \frac{\partial M}{\partial y} = 4xy = \frac{\partial N}{\partial x} \\ Solution is x^2y^2 + x^3 = c.
\]
\vfill


\end{document}
                
