\documentclass{article}
\usepackage{custom}
\usepackage{cancel}
\usepackage{shortex}
\title{Chapter 5}

\setcounter{section}{5}

\begin{document}

\maketitle
\pagebreak

\subsection{Eigen Vectors. Eigen Vectors}

\bdefn

\[
    A\vec{x} = \lambda \vec{x}
\]

$\lambda$ can be $\pm$, 0, or complex.
This is known as the eigen value.

The eigen vector, $\vec{x}$, where $\vec{x} \ne 0$

\edefn

\subsubsection{Examples}

\subsubsection*{2}

\[
    \det (\lambda I - A) = 0
\]

\bcent
This is the characteristic equation; yes the same one from diff eq!
\ecent 

\[
    a = \begin{bmatrix} 
    5 & -1 \\ 1 & 3
\end{bmatrix} && \vec{x} = \begin{bmatrix} 
1 \\ 1
\end{bmatrix}
\]

\[
    &\begin{bmatrix} 
    5 \\ 1
    \end{bmatrix} + \begin{bmatrix} 
    -1 \\ 3
    \end{bmatrix} \\
    = &\begin{bmatrix} 
    4 \\ 4
    \end{bmatrix} = 4 \begin{bmatrix} 
    1 \\ 1
    \end{bmatrix}
\]
\[
    \lambda = 4 && \vec{x} = \begin{bmatrix} 
    1 \\ 2
    \end{bmatrix}
\]

\subsubsection*{5 d)}

\[
    \begin{bmatrix} 
    1 & -2 \\ 0 & 1
    \end{bmatrix}
\]

\[
    \lambda = ?
\]

\[
    &\det(\lambda I - A) = 0 \\
    &\det\lt(\begin{bmatrix} 
    \lambda & 0 \\ 0 & \lambda
    \end{bmatrix} - \begin{bmatrix} 
    1 & -2 \\ 0 & 1
    \end{bmatrix}\rt) = 0 \\
    &\det \begin{bmatrix} 
    \lambda - 1 & 2 \\ 0  \lambda-1
    \end{bmatrix} = 0 \\
    &(\lambda - 1)^{2} = 0 \\
    &\lambda = 1,1
\]

\subsubsection*{8}

\(
    \begin{bmatrix} 1 & 0 & -2 \\ 0 & 0 & 0 \\ -2 & 0 & 4\end{bmatrix} \\
\)

\[
    \begin{vmatrix} \lambda-1 & 0 & 2 \\ 0 & \lambda & 0 \\ 2 & 0 & \lambda - 4 \end{vmatrix} &= \\
                              &= (\lambda - 1)(\lambda)(\lambda-4) - 4\lambda \\ 
                              &= \lambda (\lambda^{2} - 5\lambda + \cancel{4} - \cancel{4}) \\
                              &= \lambda^{2} (\lambda - 5) \\
\]

\(
    \lambda = 0,\ ,0\ ,5
\)

\[
    \lambda = 0 && \begin{bmatrix} -1 & 0 & 2 \\ 0 & 0 & 0 \\ 2 & 0 & -4\end{bmatrix} \begin{bmatrix} x_{1} \\ x_{2} \\ x_{3}\end{bmatrix} = \begin{bmatrix} 0 \\ 0 \\ 0\end{bmatrix}
\]

\[
    -x_{1} + 2x_{3} = 0 && x_{1} = 2x_{3} && x_{3} = t \\
    x_{2} = s && && x_{1} = 2t \\
\]

\[
    \begin{bmatrix} x_{1} \\ x_{2} \\ x_{3} \end{bmatrix} = \begin{bmatrix} 2t \\ s \\ t \end{bmatrix} = t \begin{bmatrix} 2 \\ 0 \\ 1 \end{bmatrix} + s \begin{bmatrix} 0 \\ 1 \\ 0 \end{bmatrix}
\]

\[
    \lambda = 5 && \begin{bmatrix} 4  & 0  & 2 \\ 0 & 5 & 0 \\ 2 & 0 & 1 \end{bmatrix} \begin{bmatrix} x_{1} \\ x_{2} \\ x_{3} \end{bmatrix} = \begin{bmatrix} 0 \\ 0 \\ 0\end{bmatrix} \\ 
    \vdots
    \begin{bmatrix} \frac{-1}{2} \\ 0 \\ 1 \end{bmatrix} \
\]

\subsubsection*{36}

\[
    \begin{bmatrix} -2 & 2 & 3 \\ -2 & 3 & 2 \\ -4 & 2 & 5 \end{bmatrix}
\]

\[
    \det(\lambda I - A) &= \det\lt(\begin{bmatrix} \lambda + 2 & -2 & -3 \\ 2 & \lambda - 3 & -2 \\ 4 & -2 & \lambda - 5 \end{bmatrix}\rt) \\
                        &= (\lambda + 2)(\lambda - 3)(\lambda - 5) + 16 + 12 - (-12(\lambda + 2) - 4(\lambda - 3) + 4(\lambda - 5))
\]



\end{document}
