
\documentclass[fleqn]{article}
\usepackage{amsmath}
\usepackage{shortex}
\title{1-4}
\begin{document}

\maketitle
\pagebreak
Verify that the matricies and scalars satisfy the stated properties. \[A = \begin{bmatrix} 3 & -1 \\ 2 & 4 \end{bmatrix}  \quad B = \begin{bmatrix} 0 & 2 \\ 1 & -4 \end{bmatrix} C = \begin{bmatrix} 4 & 1 \\ -3 & -2 \end{bmatrix}  \quad a = 4  \quad b = -7 \]

\subparagraph{3}

\[
(a) (A^T)^T = A (b) (AB)^T = B^T A^T
\]
\vfill



\subparagraph{4}

\[
(a) (A + B)^T = A^T + B^T (b) (aC)^T = aC^T
\]
\vfill


\pagebreak
 Compute the inverse of the matrix.

\subparagraph{5}

\[
A = \begin{bmatrix} 2 & -3 \\ 4 & 4 \end{bmatrix}
\]
\vfill



\subparagraph{7}

\[
C = \begin{bmatrix} 2 & 0 \\ 0 & 3 \end{bmatrix}
\]
\vfill


\pagebreak


\subparagraph{9}

\[
\begin{bmatrix} \frac{1}{2}(e^{x}+e^{-x}) & \frac{1}{2}(e^{x}-e^{-x})\\ \frac{1}{2}(e^{x}-e^{-x}) & \frac{1}{2}(e^{x}+e^{-x}) \end{bmatrix}
\]
\vfill

 Verify that the equation is valid for \[A = \begin{bmatrix} 2 & -3 \\ 4 & 4 \end{bmatrix} \\ B = \begin{bmatrix} 3 & 1 \\ 5 & 2 \end{bmatrix} \\ C = \begin{bmatrix} 2 & 0 \\ 0 & 3 \end{bmatrix} \\ D = \begin{bmatrix} 6 & 4 \\ -2 & -1 \end{bmatrix} \]

\subparagraph{13}

\[
(ABC)^{-1} = C^{-1}B^{-1}A^{-1}
\]
\vfill


\pagebreak
 Find $A$.

\subparagraph{15}

\[
 (7A)^{-1} = \begin{bmatrix} -3 & 7\\ 1 & -2 \end{bmatrix}
\]
\vfill

 Compute the given equation using $A$.

\subparagraph{19 a)}

\[
    A &= \begin{bmatrix} 3 & 1 \\ 2 & 1 \end{bmatrix} \\ A^3 &= ?
\]
\vfill


\pagebreak


\subparagraph{b)}

\[
 A^{-3}
\]
\vfill

 Compute $p(A)$ for the given functions: \[a) \quad p(x) = x - 2\\b) \quad p(x) = 2x2 - x + 1\\c) \quad p(x) = x3 - 2x + 1\]

\subparagraph{21}

\[
A = \begin{bmatrix} 3 & 1 \\ 2 & 1 \end{bmatrix}
\]
\vfill


\pagebreak
Show that if a square matrix $A$ satisfies the equation $A^2 + 2A + I = 0$, then $A$ must be invertible. What is the inverse?

\subparagraph{33 a)}

\[
\]
\vfill

 In Exercises 37â€“38  determine whether A is invertible  and if so  find the inverse. [Hint: Solve AX = I for X by equating corresponding entries on the two sides.]

\subparagraph{39}

\[
(AB)^{-1}(AC^{-1})(D^{-1}C^{-1})^{-1}D^{-1}
\]
\vfill


\pagebreak


\subparagraph{43 a)}

Show that if A is invertible and AB = AC, then B = C.
\vfill


\end{document}
                
