
\documentclass[fleqn]{article}
\usepackage{amsmath}
\usepackage{shortex}
\title{1-8}
\begin{document}

\maketitle
\pagebreak
 Find the domain and comdomain of the transformation $T_A(x) = Ax$.

\subparagraph{1 a)}

\[
A\text{ has size }3 \times 2.
\]
\vfill

 Find the domain and codomain defined by the equations.

\subparagraph{3 b)}

\[
\begin{aligned} w_1 &= 5x_1 - 7x_2 \\ w_2 &= 6x_1 + x_2 \\ w_3 &= 2x_1 + 3x_2 \end{aligned}
\]
\vfill


\pagebreak
 Find the domain and codomain of the transformation defined by the matrix product.

\subparagraph{5 a)}

\[
\begin{bmatrix} 3 & 1 & 2 \\ 6 & 7 & 1 \end{bmatrix} \begin{bmatrix} x_1 \\ x_2 \\ x_3 \end{bmatrix}
\]
\vfill

 Find the domain and codomain of the transformation $T$ defined by the equations.

\subparagraph{7 a)}

\[
T(x_1, x_2) = (2x_1 - x_2, x_1 + x_2)
\]
\vfill


\pagebreak


\subparagraph{9}

\[
T\left(\begin{bmatrix}x_1\\x_2\end{bmatrix}\right) = \begin{bmatrix}4x_1\\x_1-x_2\\3x_2\end{bmatrix}
\]
\vfill

Find the standard matrix for the operator $T: R^3 \to R^3$ defined by, 
\[ 
    w_1 = 3x_1 + 5x_2 - x_3 \\ w_2 = 4x_1 - x_2 + x_3 \\ w_3 = 3x_1 + 2x_2 - x_3 
\] 

and then compute $T(-1, 2, 4)$ by directly sustituing the equations and then by matrix multiplication.

\subparagraph{15}

\vfill

\pagebreak
 "In Exercises 17â€“18  find the standard matrix for the transformation and use it to compute $T(\mathbf{x})$. Check your result by substituting directly in the formula for $T$."

\subparagraph{17}

\[
    (a) && T(x_1, x_2) = (-x_1 + x_2, x_2); && \mathbf{x} = (-1, 4)\\(b) && T(x_1, x_2, x_3) = (2x_1 - x_2 + x_3, x_2 + x_3, 0); && \mathbf{x} = (2, 1, -3)
\]
\vfill

 Find $T_A(x)$ and express your answer in matrix form.

\subparagraph{19 b)}

\[
A = \begin{bmatrix} -1 & 2 & 0 \\ 3 & 1 & 5 \end{bmatrix}; \ \mathbf{x} = \begin{bmatrix} -1 \\ 1 \\ 3 \end{bmatrix}
\]
\vfill


\pagebreak
 Show that $T$ is a matrix transformation but using the previous Theorem of homogenaity and linear transformation.

\subparagraph{21 a)}

\[
T(x, y) = (2x + y, x - y)
\]
\vfill

 Show that $T$ is not a matrix transformation.

\subparagraph{23 a)}

\[
T(x, y) = (x^2, y)
\]
\vfill


\pagebreak

\end{document}
                
